Progress on debugging Blake2 experiment

specs/Spec.Blake2.Incremental.fst
@@ -9,7 +9,7 @@ open Lib.LoopCombinators
 open Spec.Blake2
 
 
-#set-options "--z3rlimit 50"
+#set-options "--z3rlimit 100"
 
 
 let max_size64_t = pow2 64 - 1
@@ -18,6 +18,7 @@ type size64_nat = n:nat{n <= max_size64_t}
 
 noeq type state_r (a:alg) = {
   hash: hash_ws a; // Current hash state
+  kk: size_nat;
   n: size_nat; // Number of blocks already processed
   pl: pl:size_nat{pl <= size_block a}; // Partial length of the block
   block: block_s a; // Storage block
@@ -26,22 +27,21 @@ noeq type state_r (a:alg) = {
 
 val blake2_incremental_init:
     a:alg
-  -> kk:size_nat{kk <= max_key a}
-  -> k:lbytes kk
+  -> k:bytes{length k <= max_key a}
   -> nn:size_nat{1 <= nn /\ nn <= max_output a} ->
   Tot (state_r a)
 
-let blake2_incremental_init a kk k nn =
+let blake2_incremental_init a k nn =
+  let kk = length k in
   let hash = blake2_init a kk k nn in
   let block = create (size_block a) (u8 0) in
-  let n = if kk = 0 then 0 else 1 in
   {
     hash = hash;
-    n = n;
+    kk = kk;
+    n = 0;
     pl = 0;
     block = block;
   }
-
 
 
 val blake2_incremental_update:
@@ -52,30 +52,36 @@ val blake2_incremental_update:
 
 let blake2_incremental_update a input state =
   let ll = length input in
-  if not (state.n + 2 + ll / size_block a <= max_size_t) then None else (
-  let br = size_block a - state.pl in
-  let ll0 = if ll <= br then ll else br in
+  let nll = ll / size_block a in
+  let nk = if state.kk = 0 then 0 else 1 in
+  if not (state.n + nk + nll + 2 <= max_size_t) then None else (
+  (* Compute the remainder space in the block *)
+  let rb = size_block a - state.pl in
+  (* Fill the partial block in the state *)
+  let ll0 = if ll < rb then ll else rb in
   let input0 = sub #uint8 #ll input 0 ll0 in
   let block: block_s a = update_sub state.block state.pl ll0 input0 in
-  if ll <= br then Some ({state with pl = state.pl + ll0; block = block})
+  let pl = state.pl + ll0 in
+  (* If the partial block is not filled *)
+  if pl < size_block a then Some ({state with pl = pl; block = block})
   else (
-    (* Handle the first partial block *)
-    let hash = blake2_update_block a (state.n * (size_block a)) block state.hash in
-    let n = state.n + 1 in
+    (* Handle the completed "partial" block *)
+    let n0 = nk + state.n in
+    let hash = blake2_update_block a ((n0 + 1) * size_block a) block state.hash in
     (* Handle all full blocks available *)
     let n1 = (ll - ll0) / size_block a in
     let ll1 = n1 * size_block a in
+    let ll2 = (ll - ll0) % size_block a in
     let input1 = sub #uint8 #ll input ll0 ll1 in
     let hash = repeati n1 (fun i ->
-      let block = sub input1 (i * size_block a) (size_block a) in
-      blake2_update_block a ((n + i) * size_block a) block)
-      hash
+        let block = sub #uint8 #(length input1) input1 (i * size_block a) (size_block a) in
+        blake2_update_block a (((n0 + 1) + i + 1) * size_block a) block
+      ) state.hash
     in
     (* Store the remainder *)
-    let ll2 = (ll - ll0) % size_block a in
     let input2 = sub #uint8 #ll input (ll - ll2) ll2 in
     let block = update_sub block 0 ll2 input2 in
-    Some ({state with n = n + n1; pl = ll2; block = block})
+    Some ({state with n = n0 + n1; pl = ll2; block = block})
   ))
 
 
@@ -90,7 +96,8 @@ let blake2_incremental_finish a state nn =
   let empty = create 0 (u8 0) in
   let last = sub state.block 0 state.pl in
   // Not very efficient because a full block will be recreated from the partial input
-  let hash = blake2_update_last a (state.n * (size_block a) + state.pl) state.pl last state.hash in
+  let nk = if state.kk = 0 then 0 else 1 in
+  let hash = blake2_update_last a ((nk + state.n) * size_block a + state.pl) state.pl last state.hash in
   blake2_finish a hash nn
 
 
@@ -104,17 +111,17 @@ let blake2_incremental_finish a state nn =
 val debug_blake2_incremental:
     a:alg
   -> d:bytes{length d <= max_size_t}
-  -> kk:size_nat{kk <= max_key a /\ (if kk = 0 then length d <= max_limb a else length d + (size_block a) <= max_limb a)}
-  -> k:lbytes kk
+  -> k:bytes{length k <= max_key a /\ (if length k = 0 then length d <= max_limb a else length d + size_block a <= max_limb a)}
   -> nn:size_nat{1 <= nn /\ nn <= max_output a} ->
   Tot (option (lbytes nn))
 
-let debug_blake2_incremental a d kk k nn =
+let debug_blake2_incremental a d k nn =
   let size_pblock = size_block a - 7 in
+  let kk = length k in
   let nd = length d / size_pblock in
   let rd = length d % size_pblock in
   let plast = sub #uint8 #(length d) d (nd * size_pblock) rd in
-  let st = blake2_incremental_init a kk k nn in
+  let st = blake2_incremental_init a k nn in
   match repeati nd (fun i ost ->
     let pinput = sub #uint8 #(length d) d (i * size_pblock) size_pblock in
     match ost with
